add small lemma about doubling range

ehoare/fast_dice.ec
@@ -57,7 +57,26 @@ rewrite H'. simplify. case (CondUnif.k{hr} <= CondUnif.n{hr}). move => H''. appl
  CondUnif.n{hr} <= CondUnif.m{hr} /\ 0 <= CondUnif.k{hr}).
  move => H. simplify. smt. smt. qed. 
  
+op indFnD (m k y : int) : real = if (1 <= m /\ 0 <= k /\ k <= 2*m -1) then (if k = y then 1.0 else 0.0) else 0.0. 
 
+module Doub_rng = {
+var m : int
+var y : int
+var x : int  
+var k : int  
+proc f() : unit = {
+    
+  x <$ [0..1];
+  y <$ [0..(m - 1)];  
+  y <- (2 * y) + x;  
+      
+}}.
+
+
+
+ehoare doub : Doub_rng.f : (((1 <= Doub_rng.m) /\ (0 <= Doub_rng.k)/\ Doub_rng.k <= (2*Doub_rng.m - 1)) `|` (1.0%xr/(2*Doub_rng.m)%xr )) ==> (indFnD Doub_rng.m Doub_rng.k Doub_rng.y)%xr.
+proof. proc. wp.  auto. progress.  case ( (1 <= Doub_rng.m{hr} /\
+   0 <= Doub_rng.k{hr} /\ Doub_rng.k{hr} <= 2 * Doub_rng.m{hr} - 1)). move => H. simplify. (* Every k corresponds to a unique pair (x,y) satisfying the equation k = 2*y + x and vice versa. Since x,y come from independent distributions, the corresponding probability is 1/2m.*) admitted.
 (*
 FDR (n) =
 v <- 1; c <- 0;
@@ -75,5 +94,6 @@ c <- c - n ;
 
 v <- 2v ;
 c <- 2c + flip() *)
+
 
 
